modify memory of FlatImp to only allow reads/writes aligned by 4 or 8 bytes
because exposing these unused lower bits to FlatImp can be useful,
and it would be annoying and inefficient to shift each memory
address in the compiler (and undo after the read/write, too)

src/FlatImp.v
@@ -1,4 +1,5 @@
 Require Import lib.LibTacticsMin.
+Require Import riscv.RiscvBitWidths.
 Require Import compiler.Common.
 Require Import compiler.Tactics.
 Require Import compiler.Op.
@@ -8,23 +9,23 @@ Require Import compiler.NameWithEq.
 
 Section FlatImp1.
 
-  Context {w: nat}. (* bit width *)
+  Context {Bw: RiscvBitWidths}.
 
   Context {Name: NameWithEq}.
   Notation var := (@name Name).
   Existing Instance eq_name_dec.
 
   Context {state: Type}.
-  Context {stateMap: Map state var (word w)}.
+  Context {stateMap: Map state var (word wXLEN)}.
   Context {vars: Type}.
   Context {varset: set vars var}.
 
-  Ltac state_calc := state_calc_generic (@name Name) (word w).
+  Ltac state_calc := state_calc_generic (@name Name) (word wXLEN).
 
   Inductive stmt: Set :=
     | SLoad(x: var)(a: var): stmt
     | SStore(a: var)(v: var): stmt
-    | SLit(x: var)(v: word w): stmt
+    | SLit(x: var)(v: word wXLEN): stmt
     | SOp(x: var)(op: binop)(y z: var): stmt
     | SSet(x y: var): stmt
     | SIf(cond: var)(bThen bElse: stmt): stmt
@@ -47,7 +48,7 @@ Section FlatImp1.
 
   (* If we want a bigstep evaluation relation, we either need to put
      fuel into the SLoop constructor, or give it as argument to eval *)
-  Fixpoint eval_stmt(f: nat)(st: state)(m: mem w)(s: stmt): option (state * mem w) :=
+  Fixpoint eval_stmt(f: nat)(st: state)(m: mem)(s: stmt): option (state * mem) :=
     match f with
     | 0 => None (* out of fuel *)
     | S f => match s with
@@ -229,18 +230,18 @@ Ltac invert_eval_stmt :=
 
 Section FlatImp2.
 
-  Context {w: nat}. (* bit width *)
+  Context {Bw: RiscvBitWidths}.
 
   Context {Name: NameWithEq}.
   Notation var := (@name Name).
   Existing Instance eq_name_dec.
 
   Context {state: Type}.
-  Context {stateMap: Map state var (word w)}.
+  Context {stateMap: Map state var (word wXLEN)}.
   Context {vars: Type}.
   Context {varset: set vars var}.
 
-  Ltac state_calc := state_calc_generic (@name Name) (word w).
+  Ltac state_calc := state_calc_generic (@name Name) (word wXLEN).
 
   Lemma increase_fuel_still_Success: forall fuel1 fuel2 initialSt initialM s final,
     fuel1 <= fuel2 ->
@@ -287,9 +288,12 @@ Section FlatImp2.
 
 End FlatImp2.
 
+Require riscv.RiscvBitWidths32.
 
 Module TestFlatImp.
 
+Import riscv.RiscvBitWidths32.
+  
 Instance ZName: NameWithEq := {| name := Z |}.
 
 Definition var: Set := (@name ZName). (* only inside this test module *)
@@ -310,8 +314,10 @@ loop:
   a = b
   b = s
   n = n - one
-*)
-Example fib(n: word 8) :=
+ *)
+
+
+Example fib(n: word 32) :=
   SSeq (SLit _one $1) (
   SSeq (SLit _n n) (
   SSeq (SLit _a $0) (
@@ -324,10 +330,10 @@ Example fib(n: word 8) :=
               (SOp _n OMinus _n _one)))))
   )))).
 
-Definition eval_stmt_test fuel initialSt := @eval_stmt 8 ZName _ _ fuel initialSt (no_mem 8).
+Definition eval_stmt_test fuel initialSt := @eval_stmt _ ZName _ _ fuel initialSt no_mem.
 
 Example finalFibState(n: nat) := (eval_stmt_test 100 empty (fib $n)).
-Example finalFibVal(n: nat): option (word 8) := match finalFibState n with
+Example finalFibVal(n: nat): option (word 32) := match finalFibState n with
 | Some (s, _) => get s _b
 | _ => None
 end.
