src/Memory.v
@@ -1,25 +1,32 @@
 Require Import bbv.Word.
+Require Import riscv.RiscvBitWidths.
 Require Import compiler.Common.
+
+Local Open Scope Z.
 
 Section Memory.
 
-  Variable w: nat. (* bit width of addresses and memory words *)
+  Context {Bw: RiscvBitWidths}.
 
-  Definition mem := word w -> option (word w).
+  Definition mem := word wXLEN -> option (word wXLEN).
 
-  Definition read_mem(x: word w)(m: mem): option (word w) := m x.
+  Definition wXLEN_in_bytes: Z :=
+    match bitwidth with
+    | Bitwidth32 => 4
+    | Bitwidth64 => 8
+    end.
+  
+  Definition read_mem(x: word wXLEN)(m: mem): option (word wXLEN) :=
+    if dec ((wordToZ x) mod (wXLEN_in_bytes) = 0) then m x else None.
 
-  Definition write_mem(x: word w)(v: word w)(m: mem): option (mem) :=
-    match m x with
+  Definition write_mem(x: word wXLEN)(v: word wXLEN)(m: mem): option (mem) :=
+    match read_mem x m with
     | Some old_value => Some (fun y => if dec (x = y) then Some v else m y)
     | None => None
     end.
 
   Definition no_mem: mem := fun x => None.
 
-  Definition zeros_mem(upTo: word w): mem := fun x => if wlt_dec x upTo then Some $0 else None.
+  Definition zeros_mem(upTo: word wXLEN): mem := fun x => if wlt_dec x upTo then Some $0 else None.
 
 End Memory.
-
-Arguments read_mem {_} _.
-Arguments write_mem {_} _ _.
